start chacha20 proof

timing/examples/crypto/chacha20/binary/build/verif_chacha.c.d
@@ -1,0 +1,1 @@
+build/verif_chacha.c.o: verif_chacha.c
