timing/examples/crypto/chacha20/chacha20_proof.v
@@ -1,16 +1,15 @@
 Require Import ChaCha20.
 Require Import RISCVTiming.
 Import RISCVNotations.
-Require Import FunctionalExtensionality.
 
 Module TimingProof (cpu : CPUTimingBehavior).
 
 Module Program_ChaCha20 <: ProgramInformation.
-    Definition entry_addr : N := 0x10c00.
+    Definition entry_addr : N := 0x224.
 
     Definition exits (t:trace) : bool :=
         match t with (Addr a,_)::_ => match a with
-        | 0x10ce4 | 0x10ce8 => true
+        | 0xcc0 => true
         | _ => false
     end | _ => false end.
 
@@ -21,427 +20,321 @@ Module RISCVTiming := RISCVTiming cpu Program_ChaCha20.
 Module ChaCha20Auto := RISCVTimingAutomation RISCVTiming.
 Import Program_ChaCha20 ChaCha20Auto.
 
-Section Invariants.
+Definition time_of_chacha20_quarter : N :=
+  tadd + txor + tslli 0x10 +
+  tadd + txor + tslli 0xc +
+  tadd + txor + tslli 0x8 +
+  tadd + txor + tsw + tslli 0x7 +
+  tsw + tsw + tjalr.
 
-  Variable sp : N               (* initial stack pointer *).
-  Variable mem : memory         (* initial memory state *).
-  Variable plaintext : addr     (* chacha20_encrypt: 1st pointer arg (R_A0) *).
-  Variable ciphertext : addr    (* chacha20_encrypt: 2nd pointer arg (R_A1) *).
-  Variable len : N              (* chacha20_encrypt: 3rd arg (R_A2) *).
-  Variable key : addr           (* chacha20_encrypt: 4th arg (R_A3) *).
-  Variable nonce : addr         (* chacha20_encrypt: 5th arg (R_A4) *).
-  Variable counter : addr       (* chacha20_encrypt: 6th arg (R_A5) *).
+Definition time_of_chacha20_block (t : trace) : Prop :=
+  cycle_count_of_trace t = taddi + 13 * tsw + 4 * taddi +
+      4 * (tsw + tlui + taddi) + 
+      8 * (tsw + taddi + 4 * tlbu + 4 * tsb + tlw) +
+      tsw + 4 * tlbu + 4 * tsb + tlw + 
+      2 * (taddi + 4 * tlbu + 4 * tsb + tlw) +
+      4 * taddi + 10 * tsw + taddi + tsw + tsw +
+      10 * (4 * taddi + 3 * tlw + tjal +
+        time_of_chacha20_quarter +
+        5 * taddi + 3 * tlw + tjal +
+        time_of_chacha20_quarter +
+        tsw + 6 * taddi + 3 * tlw + tjal +
+        time_of_chacha20_quarter +
+        8 * taddi + 3 * tlw + tjal +
+        time_of_chacha20_quarter +
+        4 * taddi + 3 * tlw + tjal +
+        time_of_chacha20_quarter +
+        5 * taddi + 3 * tlw + tjal +
+        time_of_chacha20_quarter +
+        4 * taddi + 4 * tlw + tjal +
+        time_of_chacha20_quarter +
+        5 * taddi + 3 * tlw + tjal +
+        time_of_chacha20_quarter + 
+        taddi + taddi) + 9 * ttbne + tfbne +
+    172 * tsb + 108 * tlbu + 65 * tlw +
+    16 * (tsrli 0x8 + tsrli 0x10 + tsrli 0x18) +
+    16 * tadd + 16 * txor + 7 * taddi + 
+    4 * tlui + tjalr.
 
-  Definition time_of_chacha20_block : N := 0.
+Definition ChaCha20_timing_invs (t:trace) : option Prop :=
+match t with (Addr a, s) :: t' => match a with
+| 0x224 => Some (cycle_count_of_trace t' = 0)
+| 0x4b8 => Some (1 <= s R_S3 <= 10 /\
+    cycle_count_of_trace t' = taddi + 13 * tsw + 4 * taddi +
+        4 * (tsw + tlui + taddi) + 
+        8 * (tsw + taddi + 4 * tlbu + 4 * tsb + tlw) +
+        tsw + 4 * tlbu + 4 * tsb + tlw + 
+        2 * (taddi + 4 * tlbu + 4 * tsb + tlw) +
+        4 * taddi + 10 * tsw + taddi + tsw + tsw +
+        (10 - s R_S3) * (4 * taddi + 3 * tlw + tjal +
+          time_of_chacha20_quarter +
+          5 * taddi + 3 * tlw + tjal +
+          time_of_chacha20_quarter +
+          tsw + 6 * taddi + 3 * tlw + tjal +
+          time_of_chacha20_quarter +
+          8 * taddi + 3 * tlw + tjal +
+          time_of_chacha20_quarter +
+          4 * taddi + 3 * tlw + tjal +
+          time_of_chacha20_quarter +
+          5 * taddi + 3 * tlw + tjal +
+          time_of_chacha20_quarter +
+          4 * taddi + 4 * tlw + tjal +
+          time_of_chacha20_quarter +
+          5 * taddi + 3 * tlw + tjal +
+          time_of_chacha20_quarter + 
+          taddi + taddi + ttbne)
+  )
+| 0xcc0 => Some (time_of_chacha20_block t)
+| _ => None end | _ => None end.
 
-  Definition time_of_chacha20_encrypt (s:store) : N :=
-    if len =? 0 then ttbeq + tjalr else
-      tfbeq + taddi + (10 * tsw) + (8 * taddi) + tjal + (6 * taddi).
-      (* time_of_chacha20_block +
-      tsub +
-      if (0 >=? ) *)
-
-  (* Invariant sets f for multi-subroutine properties have the following signature:
-        f (T:Type) (Invs Post: inv_type T) (NoInv:T) (s:store) (a:addr) : T
-     where inv_type T = N -> Prop -> T.  They thereby map addresses a:addr to
-     internal invariants (Invs n P), post-conditions (Post n P), or no-invariant (NoInv),
-     where n:N is a subroutine identifier number and P:Prop is the invariant.
-     Polymorphic parameters Invs, Post, and NoInv act like constructors of return type T.
-     Property P usually references store s, and is therefore a property of s.
-     Identifiers n are unique to each subroutine in the code, and establish a
-     partial order over subroutines:  A caller with identifier m may use Picinae's
-     perform_call theorem to call a callee with identifier n whenever m > n.
-     (To verify mutually recursive nests of subroutines, they must be assigned a
-     common identifier and verified as a single recursive subroutine.)
-
-     Note that because of the "Variable" declarations above, the following invariant
-     set definition "invs" actually has extra initial hidden parameters, one for each
-     sectional Variable it references:
-       invs sp mem raddr ... T Inv Post NoInv s a
-     It therefore actually defines an invariant set family, one invariant set for each
-     possible instantiation of the Variable parameters before T.  To allow a caller to
-     call a callee with a different invariant set from the same family using perform_call,
-     the two invariant sets f and g must satisfy (same_invset_family f g), which stipulates
-     that f and g agree on whether an internal invariant or post-condition exists at each
-     address, though they may differ on what the invariant P is.  The same_invset_family
-     obligation is provable by reflexivity as long as your definition only refers to
-     (hidden) parameters before T within the P arguments of Inv and Post. *)
-  Definition invs T (Inv Post: inv_type T) (NoInv:T) (s:store) (a:addr) : T :=
-    match a with
-    (* strcasecmp entry point *)
-    | 1048576 => Inv 1 (
-        s R_SP = sp /\ s V_MEM64 = mem /\
-        s R_X0 = arg1 /\ s R_X1 = arg2
-      )
-
-    (* loop invariant *)
-    | 1048600 => Inv 1 (∃ fb k,
-        strcaseeq (mem' fb) arg1 arg2 k /\
-        s R_SP = sp ⊖ 48 /\ s V_MEM64 = mem' fb /\
-        s R_X19 = arg2 ⊕ k /\ s R_X20 = arg1 ⊕ k
-      )
-
-    (* case-equal, non-null characters found *)
-    | 1048688 => Inv 1 (∃ fb k,
-        strcaseeq (mem' fb) arg1 arg2 k /\
-        s R_SP = sp ⊖ 48 /\ s V_MEM64 = mem' fb /\
-        s R_X19 = arg2 ⊕ k /\ s R_X20 = arg1 ⊕ k /\
-        (tolower(mem' fb Ⓑ[arg1 + k]) = tolower(mem' fb Ⓑ[arg2 + k])) /\
-        mem' fb Ⓑ[arg1 + k] ≠ 0
-      )
-
-    (* case-unequal or null characters found *)
-    | 1048648 => Inv 1 (∃ fb k,
-        strcaseeq (mem' fb) arg1 arg2 k /\ (*characters before k matched*)
-        s R_SP = sp ⊖ 48 /\ s V_MEM64 = mem' fb /\
-        s R_X19 = arg2 ⊕ k /\ s R_X20 = arg1 ⊕ k /\
-          (tolower(mem' fb Ⓑ[arg1 + k]) ≠ tolower(mem' fb Ⓑ[arg2 + k]) \/
-           mem' fb Ⓑ[arg1 + k] = 0)
-      )
-
-    (* strcasecmp return site *)
-    | 1048684 => Post 1 (postcondition s)
-
-    (* tolower entry point *)
-    | 2097152 => Inv 0 (s R_X0 = arg1 /\ s R_X19 = arg2 /\
-         s R_X20 = x20 /\ s R_X21 = x21 /\
-         s R_X30 = raddr /\ s R_SP = sp /\ s V_MEM64 = mem)
-
-    (* tolower return point *)
-    | 2097168 => Post 0 (s R_X0 = tolower arg1 /\ s R_X19 = arg2 /\
-         s R_X20 = x20 /\ s R_X21 = x21 /\
-         s R_X30 = raddr /\ s R_SP = sp /\ s V_MEM64 = mem)
-
-    | _ => NoInv
+Local Ltac step := tstep r5_step.
+(* "Forget" step - throw away the store after each step
+    This is convenient for many segments of ChaCha in which functional
+    semantics do not affect timing or control flow at all
+*)
+Local Ltac fstep := step; 
+    match goal with
+    | [old_s : store |- context[(Addr _, update ?old_s _ _) :: _]] =>
+        let trash := fresh "s''" in
+        rename old_s into trash;
+        match goal with [|- context[update trash ?k ?v]] =>
+          set (old_s := update trash k v)
+        end;
+        try match goal with [ACC: MemAcc _ _ _ _ _ |-_] =>
+          clear ACC
+        end;
+        clearbody old_s;
+        try clear trash
     end.
 
-  (* Picinae's helper functions make_exits and make_invs are next leveraged to
-     define appropriate invariant sets for each subroutine by extracting them
-     from the above.  Note that these definitions receive the same extra hidden
-     parameters as invs above, so are actually invariant set families. *)
-  Definition exits0 := make_exits 0 strcasecmp invs.
-  Definition invs0 := make_invs 0 strcasecmp invs.
-  Definition exits1 := make_exits 1 strcasecmp invs.
-  Definition invs1 := make_invs 1 strcasecmp invs.
+Notation "f '[U' x := y ]" := (update f x y) (at level 50, left associativity, format "f '/'  [U  x  :=  y ]").
 
-End Invariants.
+(* fstep except keep one variable in the store *)
+Local Ltac fstep_keep val := step; 
+    lazymatch goal with
+    | [old_s:store |- context[(Addr _, update (update ?old_s val _) R_RA _) :: _]] =>
+        idtac (* don't want to get rid of RA *)
+    | [old_s:store |- context[(Addr _, update (update ?old_s val _) _ _) :: _]] =>
+        rewrite update_swap by discriminate;
+        let trash := fresh "s''" in
+        rename old_s into trash;
+        match goal with [|- context[update trash ?k ?v]] =>
+          set (old_s := update trash k v)
+        end;
+        try match goal with [ACC: MemAcc _ _ _ _ _ |-_] =>
+          clear ACC
+        end;
+        clearbody old_s;
+        try clear trash
+    | [|- context[(Addr _, update _ val _) :: _]] => idtac
+    | [old_s : store |- context[(Addr _, update ?old_s _ _) :: _]] =>
+        let trash := fresh "s''" in
+        rename old_s into trash;
+        match goal with [|- context[update trash ?k ?v]] =>
+          set (old_s := update trash k v)
+        end;
+        try match goal with [ACC: MemAcc _ _ _ _ _ |-_] =>
+          clear ACC
+        end;
+        clearbody old_s;
+        try clear trash
+    end.
+
+Ltac clear_unused :=
+  repeat match goal with
+  | H : N |- _ =>
+    tryif (clear dependent H) then idtac else fail
+  | H : memory |- _ =>
+    tryif (clear dependent H) then idtac else fail
+  end.
+
+Ltac generalize_reg :=
+  repeat multimatch goal with
+  | [|- context[_ [U ?r := ?f ?x]]] =>
+    match r with
+    | R_S3 => idtac | R_RA => idtac
+    | _ => generalize (f x); intros
+    end
+  | _ => idtac
+  end;
+  clear_unused.
+
+Ltac gstep := step; generalize_reg.
+
+Theorem ChaCha20_timing:
+  forall s (t : trace) s' x'
+         (* boilerplate *)
+         (ENTRY: startof t (x',s') = (Addr entry_addr, s))
+         (MDL: models rvtypctx s),
+  satisfies_all 
+    lifted_prog
+    (ChaCha20_timing_invs)
+    exits
+  ((x',s')::t).
+Proof using.
+    intros.
+    apply prove_invs.
+
+    simpl. rewrite ENTRY. unfold entry_addr. step. reflexivity.
+
+    intros.
+    eapply startof_prefix in ENTRY; try eassumption.
+    eapply preservation_exec_prog in MDL; 
+        try eassumption; [idtac|apply lift_riscv_welltyped].
+    clear - ENTRY PRE MDL. rename t1 into t. rename s1 into s'.
+
+    destruct_inv 32 PRE.
+    - (* 0x224 -> 4b8 *)
+      admit.
+      (* repeat gstep. 
+      split.
+        lia.
+        hammer. *)
+    - (* 0x4b8 -> 0x5ec *)
+      destruct PRE as (S3 & Cycles).
+        do 206 gstep.
+          replace (s' R_S3 ⊖ 1) with (s' R_S3 - 1) in * by
+            (rewrite msub_nowrap; psimpl; lia).
+          apply Bool.negb_true_iff in BC.
+          split.
+            apply N.eqb_neq in BC. lia.
+          replace (10 - (s' R_S3 - 1)) with 
+            (1 + (10 - s' R_S3)) by lia.
+          repeat rewrite (N.mul_add_distr_r 1).
+
+          match goal with
+          |[|-context[(10 - _) * ?x]] =>
+            remember x as loop_body_time
+          end.
+
+          (* Ltac recurse_add x :=
+            match x with
+            | N.add ?a ?b => recurse_add a; idtac " +" b
+            | _ => idtac x
+            end.
+          match goal with
+          | [|- context[?x + ?y]] => recurse_add (x + y)
+          end. *)
+
+          remember (10 - s' R_S3).
+          hammer. psimpl.
+
+          Ltac append l1 l2 :=
+            lazymatch l1 with
+            | [] => l2
+            | ?x :: ?xs =>
+                let tail := append xs l2 in
+                constr:(x :: tail)
+            end.
+
+          Ltac flatten_plus t :=
+            lazymatch t with
+            | ?a + ?b =>
+                let la := flatten_plus a in
+                let lb := flatten_plus b in
+                append la lb
+            | ?x => constr:([x])
+            end.
 
 
-(* Prove a few helper lemmas about tolower and friends: *)
+          Ltac remove_once x l :=
+            lazymatch l with
+            | [] => fail "no match for" x
+            | x :: ?xs => xs
+            | ?y :: ?ys =>
+                let ys' := remove_once x ys in
+                constr:(y :: ys')
+            end.
 
-Lemma tolower_small:
-  forall w e m a, tolower (getmem w e 1 m a) < 2^8.
-Proof.
-  intros. unfold tolower. destruct (andb _ _).
-    apply lor_bound.
-      rewrite <- getmem_mod_r, mp2_mod_mod_min. apply mp2_mod_lt.
-      reflexivity.
-    apply getmem_bound.
+          Ltac multiset_match lhs rhs :=
+            lazymatch lhs with
+            | [] => 
+              match rhs with
+              | [] => idtac
+              | ?rhs' => 
+                idtac "Extras:" rhs' (* leftover RHS terms = extras *)
+              end
+            | ?x :: ?xs =>
+                tryif (let rhs' := remove_once x rhs in
+                      multiset_match xs rhs')
+                then idtac
+                else (
+                  idtac "could not find match for" x)
+            | _ => idtac lhs
+            end.
+
+          Ltac compare_sums :=
+            match goal with
+            | [|- ?lhs = ?rhs] =>
+                let L := flatten_plus lhs in
+                let R := flatten_plus rhs in
+                (* idtac L;
+                idtac R; *)
+                multiset_match L R
+                (* tryif (multiset_match L R; idtac)
+                then idtac "all terms matched"
+                else fail "mismatch between" L "and" R *)
+            end.
+
+          compare_sums.
+
+          Ltac count_occurrences x t :=
+  lazymatch t with
+  | x => constr:(1)                                (* exact match *)
+  | ?f ?a =>
+      let n1 := count_occurrences x f in
+      let n2 := count_occurrences x a in
+      let n := eval compute in (n1 + n2) in
+      constr:(n)
+  | ?a + ?b =>
+      let n1 := count_occurrences x a in
+      let n2 := count_occurrences x b in
+      let n := eval compute in (n1 + n2) in
+      constr:(n)
+  | _ => constr:(0)
+  end.
+
+  Ltac count_in_goal x :=
+  match goal with
+  | |- ?g =>
+      let n := count_occurrences x g in
+      idtac x "appears" n "time(s) in the goal"
+  end.
+
+  (* count_in_goal ttbne. *)
+  subst n6 loop_body_time.
+  unfold time_of_chacha20_quarter.
+  (* count_in_goal ttbne. *)
+  (* compare_sums. *)
+  (* count_in_goal tlw. *)
+  hammer.
+
+  (* postcondition *)
+  repeat gstep.
+
+  unfold time_of_chacha20_quarter.
+  hammer.
+  unfold time_of_chacha20_quarter.
+  apply Bool.negb_false_iff in BC.
+  apply N.eqb_eq in BC.
+  rewrite msub_nowrap in BC.
+  psimpl in BC.
+  replace (s' R_S3) with 1 in * by lia.
+  hammer.
+  compare_sums.
+  
+
+
+
+          match goal with
+          | [|- ?x = _] => let x' := (flatten_plus x) in idtac x'
+          end.
+          
+
+      (* do 205 fstep_keep R_RA. step. *)
+      -- (* Loop around *)
+        hammer.
+      
 Qed.
 
-Lemma tolower_mod:
-  forall c, (tolower c) mod 2^32 = tolower (c mod 2^32).
-Proof.
-  intro. unfold tolower. rewrite mp2_mod_mod. destruct (andb _ _).
-    rewrite <- N.land_ones, N.land_lor_distr_l, N.land_ones, mp2_mod_mod. reflexivity.
-    reflexivity.
-Qed.
-
-Lemma tolower_byte:
-  forall w e m a, (tolower (getmem w e 1 m a)) mod 2^32 =
-                  tolower (getmem w e 1 m a).
-Proof.
-  intros. rewrite tolower_mod, N.mod_small. reflexivity.
-  etransitivity. apply getmem_bound. reflexivity.
-Qed.
-
-Lemma tolower_test:
-  forall c,
-    (if 25 <=? msub 32 c 65
-     then if c mod 2^32 =? 90 then 0 else 1
-     else 0) =
-    (if andb (65 <=? c mod 2^32) (c mod 2^32 <=? 90) then 0 else 1).
-Proof.
-  intro c. destruct (N.eq_dec (c mod 2^32) 90) as [H1|H1].
-    rewrite <- (msub_mod_l 32 32). rewrite H1. reflexivity. reflexivity.
-    rewrite (proj2 (N.eqb_neq _ _) H1). destruct (65 <=? _) eqn:H2.
-      apply N.leb_le in H2. destruct (_ <=? 90) eqn:H3.
-        rewrite (proj2 (N.leb_gt _ _)).
-          reflexivity.
-          change 25 with (msub 32 90 65). apply msub_lt_mono_r.
-            left. rewrite N.min_l. apply H2. apply N.leb_le, H3.
-            apply N.leb_le, N.le_lteq in H3. destruct H3 as [H3|H3].
-              assumption.
-              contradict H1. assumption.
-        apply N.leb_gt in H3. rewrite msub_nowrap by assumption. rewrite (proj2 (N.leb_le _ _)).
-          reflexivity.
-          apply N.le_add_le_sub_l, N.lt_le_incl, H3.
-      rewrite msub_wrap by apply N.leb_gt, H2. rewrite (proj2 (N.leb_le _ _)).
-        reflexivity.
-        apply N.le_add_le_sub_l. transitivity (2^32). discriminate 1. apply N.le_add_r.
-Qed.
-
-Lemma diff_compare:
-  forall m n (H1: m < 2^8) (H2: n < 2^8),
-    (m ?= n) = (toZ 32%N (msub 32%N m n) ?= 0)%Z.
-Proof.
-  intros.
-  assert (H1': m < 2^32). eapply N.lt_le_trans. apply H1. discriminate.
-  assert (H2': n < 2^32). eapply N.lt_le_trans. apply H2. discriminate.
-  destruct (m ?= n) eqn:H3; symmetry.
-    apply N.compare_eq_iff in H3. subst. rewrite msub_diag. reflexivity.
-    apply (proj2 (Z.compare_lt_iff _ _)), Z.lt_nge.
-      intro H. apply toZ_sign in H. revert H. apply N.le_ngt.
-      rewrite msub_mod_pow2, N.min_id. apply le_msub_iff.
-      right. rewrite !N.mod_small by assumption. split.
-        apply (proj1 (N.compare_lt_iff _ _) H3).
-        transitivity (2^8+2^31).
-          apply N.add_le_mono. apply N.lt_le_incl, H2. discriminate.
-          transitivity (2^32). discriminate. apply N.le_add_r.
-    apply (proj1 (N.compare_gt_iff _ _)) in H3. apply (proj2 (Z.compare_gt_iff _ _)).
-      rewrite msub_nowrap by (rewrite !N.mod_small by assumption; apply N.lt_le_incl, H3).
-      rewrite !N.mod_small by assumption.
-      rewrite (proj1 (toZ_nonneg _ _)); rewrite N.mod_small.
-      rewrite N2Z.inj_sub by apply N.lt_le_incl, H3. apply Z.lt_0_sub, N2Z.inj_lt, H3.
-      1-3: eapply N.le_lt_trans; [apply N.le_sub_l|try assumption].
-      eapply N.lt_le_trans. apply H1. discriminate.
-Qed.
-
-(* Create a step tactic that prints a progress message (for demos). *)
-Ltac step := time arm8_step.
-
-(* Prove that each subroutine satisfies the invariant set, starting with callees
-   and proceeding to callers.  In this case, we start with subroutine tolower: *)
-Theorem tolower_correctness:
-  forall s sp mem t xs' arg1 arg2 a'
-         (ENTRY: startof t xs' = (Addr 2097152, s))
-         (MDL: models arm8typctx s)
-         (SP: s R_SP = sp) (MEM: s V_MEM64 = mem)
-         (X0: s R_X0 = arg1) (X19: s R_X19 = arg2)
-         (X30: s R_X30 = a'),
-  satisfies_all strcasecmp (invs0  sp mem a' arg1 arg2 (s R_X20) (s R_X21))
-                           (exits0 sp mem a' arg1 arg2 (s R_X20) (s R_X21)) (xs'::t).
-Proof.
-  (* Use prove_invs to initiate a proof by induction. *)
-  intros. apply prove_invs.
-
-  (* Base case: The invariant at the subroutine entry point is satisfied. *)
-  simpl. rewrite ENTRY. step. repeat split; assumption.
-
-  (* Before proving all the inductive cases (which each start at an internal
-     invariant point), clean up the proof context by replacing any hypotheses
-     about initial cpu state s with equivalent hypotheses about the cpu state s1
-     that appears at the invariant point at which we're starting this case. *)
-  intros.
-  eapply startof_prefix in ENTRY; try eassumption.
-  eapply preservation_exec_prog in MDL; try (eassumption || apply strcasecmp_welltyped).
-  clear - PRE MDL. rename t1 into t.
-
-  (* Break the proof into cases, one for each internal invariant-point. *)
-  destruct_inv 64 PRE.
-
-  (* Address 152 (tolower entry point) *)
-  destruct PRE as [X0 [X19 [X20 [X21 [X30 [SP MEM]]]]]].
-  step. step. step.
-
-    (* Address 1048164 *)
-    step. repeat split; try assumption.
-    rewrite tolower_test in BC. unfold tolower.
-    destruct (andb _ _). reflexivity. discriminate.
-
-    (* Address 104168 *)
-    repeat split; try assumption.
-    rewrite tolower_test in BC. unfold tolower.
-    destruct (andb _ _). discriminate. reflexivity.
-Qed.
-
-(* Now prove correctness of the main strcasecmp subroutine,
-   using our earlier proof of tolower at subroutine calls. *)
-Theorem strcmp_partial_correctness:
-  forall s sp mem t s' x' arg1 arg2 a'
-         (ENTRY: startof t (x',s') = (Addr 1048576, s))
-         (MDL: models arm8typctx s)
-         (SP: s R_SP = sp) (MEM: s V_MEM64 = mem) (X30: s R_X30 = a')
-         (RX0: s R_X0 = arg1) (RX1: s R_X1 = arg2),
-  satisfies_all strcasecmp (invs1  sp mem a' arg1 arg2 (s R_X20) (s R_X21))
-                           (exits1 sp mem a' arg1 arg2 (s R_X20) (s R_X21)) ((x',s')::t).
-Proof.
-  (* Use prove_invs to initiate a proof by induction. *)
-  intros. apply prove_invs.
-
-  (* Base case: The invariant at the subroutine entry point is satisfied. *)
-  simpl. rewrite ENTRY. step. repeat split; assumption.
-
-  (* Change assumptions about s into assumptions about s1. *)
-  intros.
-  eapply startof_prefix in ENTRY; try eassumption.
-  eapply preservation_exec_prog in MDL; try (eassumption || apply strcasecmp_welltyped).
-  set (x20 := s R_X20) in *. set (x21 := s R_X21) in *. clearbody x20 x21.
-  clear - PRE MDL. rename t1 into t. rename s1 into s.
-
-  (* Break the proof into cases, one for each internal invariant-point. *)
-  destruct_inv 64 PRE.
-
-  (* Address 1048576: strcasecmp entry point *)
-  destruct PRE as [MEM [SP [X0 X1]]].
-  step. step. step. step. step. step.
-  generalize_frame mem as fb.
-  exists fb, 0. psimpl. split.
-    intros i LT. destruct i; discriminate.
-    repeat split.
-
-  (* Address 1048600: strcasecmp main loop *)
-  destruct PRE as [fb [k [SEQ [SP [MEM [X19 X20]]]]]].
-  step. step.
-
-    (* Address 1048648: reached null terminator in arg1 *)
-    exists fb, k. repeat (reflexivity || assumption || split).
-    right. apply N.eqb_eq, BC.
-
-    (* Address 1048608: character in arg1 is non-null. *)
-    apply N.eqb_neq in BC.
-    step. step.
-
-      (* Address 1048648: reached null terminator in arg2 *)
-      apply N.eqb_eq in BC0.
-      exists fb, k. repeat (reflexivity || assumption || split).
-      left. rewrite BC0. change (tolower 0) with 0. unfold tolower.
-      destruct (andb _ _).
-        intro H. apply N.lor_eq_0_iff, proj2 in H. discriminate.
-        assumption.
-
-      (* Address 1048616: Current char in both strings are non-null. *)
-      apply N.eqb_neq in BC0.
-      step. step.
-
-        (* Address 1048688: identical characters found *)
-        eexists fb, k. repeat (assumption || reflexivity || split).
-        apply N.eqb_eq in BC1. rewrite BC1. reflexivity.
-
-        (* Address 1048624: Unequal characters found. Call tolower(arg1). *)
-        step.
-        set (s1 := update _ _ _).
-        eapply models_after_steps. eassumption. apply strcasecmp_welltyped. intro MDL1.
-        eapply (perform_call 0). reflexivity.
-        intros. eapply tolower_correctness; (eassumption || reflexivity).
-        reflexivity.
-
-        (* Clean up the proof context after the call by creating hypotheses
-           about the post-call cpu state s1 and discarding hypotheses about
-           old cpu states. *)
-        intros.
-        unfold s1 in PRE. psimpl in PRE.
-        assert (MDL': models arm8typctx s').
-          eapply preservation_exec_prog; try eassumption.
-          apply strcasecmp_welltyped.
-        set (t' := t2++t0++_::t) in *. clearbody s1 t'.
-        set (x21' := s R_X21) in PRE. clearbody x21'.
-        clear - SEQ BC BC0 BC1 PRE MDL'.
-        rename MDL' into MDL. rename t' into t. rename a'0 into a. rename s' into s.
-
-        (* Separate the proof into one subgoal for each subroutine exit point.
-           (In the case of tolower, there's only one exit point. *)
-        destruct_inv 64 PRE.
-
-        destruct PRE as [X0 [X19 [X20 [X21 [X30 [SP MEM]]]]]].
-        clear X21 x21'. (* This particular call site ignores x21, so delete it. *)
-        step. step. step. step.
-
-        (* Another call to tolower, performed in the same way as above. *)
-        set (s1 := update _ _ _).
-        eapply models_after_steps. eassumption. apply strcasecmp_welltyped. intro MDL1.
-        eapply (perform_call 0). reflexivity.
-        intros. eapply tolower_correctness; (eassumption || reflexivity).
-        reflexivity.
-
-        intros.
-        unfold s1 in PRE. psimpl in PRE.
-        assert (MDL': models arm8typctx s').
-          eapply preservation_exec_prog; try eassumption.
-          apply strcasecmp_welltyped.
-        set (t' := t2++t0++_::t) in *. clearbody s1 t'.
-        rewrite X20 in PRE.
-        clear - SEQ BC BC0 BC1 PRE MDL'.
-        rename MDL' into MDL. rename t' into t. rename a'0 into a. rename s' into s.
-
-        destruct_inv 64 PRE.
-
-        destruct PRE as [X0 [X19 [X20 [X21 [X30 [SP MEM]]]]]].
-        step. step. step.
-
-          (* Address 1048688: found case-equal characters *)
-          exists fb, k.
-          rewrite !tolower_byte in BC2.
-          repeat first [ assumption | split ].
-          apply N.eqb_eq, BC2.
-
-          (* Address 1048648: found case-unequal characters *)
-          exists fb, k.
-          rewrite !tolower_byte in BC2.
-          repeat first [ assumption | split ].
-          left. apply N.eqb_neq, BC2.
-
-        (* Address 1048648: case-unequal chars or null found *)
-        destruct PRE as [fb [k [SEQ [SP [MEM [X19 [X20 NEQ]]]]]]].
-        step. step.
-
-        (* Another call to tolower, performed the same as above. *)
-        set (s1 := update _ _ _).
-        eapply models_after_steps. eassumption. apply strcasecmp_welltyped. intro MDL1.
-        eapply (perform_call 0). reflexivity.
-        intros. eapply tolower_correctness; (eassumption || reflexivity).
-        reflexivity.
-
-        intros.
-        unfold s1 in PRE. psimpl in PRE.
-        set (x21' := s R_X21) in PRE. clearbody x21'.
-        assert (MDL': models arm8typctx s').
-          eapply preservation_exec_prog; try eassumption.
-          apply strcasecmp_welltyped.
-        set (t' := t2++t0++_::t) in *. clearbody s1 t'.
-        clear - SEQ NEQ PRE MDL'.
-        rename MDL' into MDL. rename t' into t. rename a'0 into a. rename s' into s.
-
-        destruct_inv 64 PRE.
-
-        destruct PRE as [X0 [X19 [X20 [X21 [X30 [SP MEM]]]]]].
-        clear X21 x21'.
-        step. step. step. step.
-
-        (* Another call to tolower, performed the same as above. *)
-        set (s1 := update _ _ _).
-        eapply models_after_steps. eassumption. apply strcasecmp_welltyped. intro MDL1.
-        eapply (perform_call 0). reflexivity.
-        intros. eapply tolower_correctness; (eassumption || reflexivity).
-        reflexivity.
-
-        intros.
-        unfold s1 in PRE. psimpl in PRE.
-        set (x21' := s R_X21) in PRE. clearbody x21'.
-        assert (MDL': models arm8typctx s').
-          eapply preservation_exec_prog; try eassumption.
-          apply strcasecmp_welltyped.
-        set (t' := t2++t0++_::t) in *. clearbody s1 t'.
-        clear - SEQ NEQ PRE MDL'.
-        rename MDL' into MDL. rename t' into t. rename a'0 into a. rename s' into s.
-
-        destruct_inv 64 PRE.
-
-        destruct PRE as [X0 [X19 [X20 [X21 [X30 [SP MEM]]]]]].
-        clear X21 x21'.
-        step. step. step. step. step.
-        eexists _, k, fb. repeat first [ reflexivity | assumption | split ].
-          intro H. apply msub_move_0_r in H. destruct NEQ as [H'|H'].
-            contradict H'. rewrite !tolower_byte in H. assumption.
-            assumption.
-          apply diff_compare; apply tolower_small.
-
-  (* Address 1048688: case-equal, non-nil chars found (loop back) *)
-  destruct PRE as [fb [k [SEQ [SP [MEM [X19 [X20 [EQ NN]]]]]]]].
-  step. step. step.
-  exists fb, (k+1). split.
-    rewrite N.add_1_r. intros i H. apply N.lt_succ_r, N.le_lteq in H. destruct H.
-      revert i H. apply SEQ.
-      subst i. split. assumption. apply N.neq_0_lt_0, NN.
-    psimpl. repeat split; assumption.
-Qed. (* <-- This Qed might take a few minutes depending on your machine. *)
+End TimingProof.
