timing/examples/crypto/chacha20/binary/build.sh
@@ -1,0 +1,1 @@
+make clean_all exe RISCV_PREFIX=/home/charles/Desktop/riscv-none-elf/bin/riscv-none-elf-
